* Move the halting problem theorems into their own theory.   Show a new one, that it is impossible to determine if phi(n,n) halts.
* Define a recursion operator termrec for terms, and in the process
  make heavy use of bracket abstraction by conditional rewriting.  If
  a definition can be re-expressed without abstractions, rewriting
  becomes a lot easier because you don't need to worry about making
  bound names fresh and all the rest of it.  This machinery will
  probably get its own theory and implementation as it's probably
  generally useful.  For the moment, it's not 100% perfect as the
  equivalence it shows is beta-equivalence, not beta-eta-equivalence,
  meaning that it blocks on 
    LAM f (LAM v (VAR f @@ VAR v))
  when it would be nice to turn it into I.  (The conditions on the
  rewrites stop the other rules from applying and turning it into
    C @@ B @@ I
  )  The answer is probably to convert all my machinery to beta-eta
  equivalence, or to allow C @@ B @@ I as a bracket abstraction of the
  lambda-term above. 

* In enumerationsScript.sml, explicitly save foo_def and foo_ind
  having used tprove to show that the definition was well-behaved.
  Irritating!

examples/lambda/computability/churchDBScript.sml
@@ -297,6 +297,248 @@ val cdLAM_behaviour = store_thm(
   SIMP_TAC (bsrw_ss()) [cdLAM_def, cdV_behaviour, cplus_behaviour, 
                         clift_behaviour, csub_behaviour, cdABS_behaviour, 
                         dLAM_def]);
+
+(* ----------------------------------------------------------------------
+    term recursion operator, termrec
+   ---------------------------------------------------------------------- *)
+
+val B_I = store_thm(
+  "B_I",
+  ``v ∉ FV M ∧ v ∈ FV N ∧ N ≠ VAR v ⇒ 
+      (LAM v (M @@ N) == B @@ M @@ (LAM v N))``,
+  STRIP_TAC THEN 
+  ASM_SIMP_TAC (bsrw_ss()) [chap2Theory.B_def] THEN 
+  REWRITE_TAC [chap2Theory.S_def] THEN 
+  Q_TAC (NEW_TAC "z") `{"x"; "y"; "z"} ∪ FV M ∪ FV N` THEN 
+  `LAM "z" (VAR "x" @@ VAR "z" @@ (VAR "y" @@ VAR "z")) = 
+   LAM z (VAR "x" @@ VAR z @@ (VAR "y" @@ VAR z))`
+     by SRW_TAC [][LAM_eq_thm] THEN 
+  POP_ASSUM SUBST1_TAC THEN 
+  Q_TAC (NEW_TAC "y") `{"x"; "y"; z} ∪ FV M ∪ FV N` THEN 
+  `LAM "y" (LAM z (VAR "x" @@ VAR z @@ (VAR "y" @@ VAR z))) =
+   LAM y (LAM z (VAR "x" @@ VAR z @@ (VAR y @@ VAR z)))`
+     by SRW_TAC [][LAM_eq_thm] THEN 
+  POP_ASSUM SUBST1_TAC THEN 
+  ASM_SIMP_TAC (bsrw_ss()) [] THEN 
+  `∀x y. (x = y) ⇒ (x == y)` by SRW_TAC [][] THEN POP_ASSUM MATCH_MP_TAC THEN 
+  SRW_TAC [boolSimps.CONJ_ss][LAM_eq_thm, tpm_fresh, NOT_IN_SUB] THEN 
+  SRW_TAC [][GSYM fresh_tpm_subst, tpm_flip_args]);
+
+val C_I = store_thm(
+  "C_I",
+  ``v ∈ FV M ∧ v ∉ FV N ⇒ LAM v (M @@ N) == C @@ (LAM v M) @@ N``,
+  STRIP_TAC THEN ASM_SIMP_TAC (bsrw_ss()) [chap2Theory.C_def] THEN 
+  REWRITE_TAC [chap2Theory.S_def] THEN 
+  Q_TAC (NEW_TAC "z") `{"x"; "y"; "z"} ∪ FV M ∪ FV N` THEN 
+  `LAM "z" (VAR "x" @@ VAR "z" @@ (VAR "y" @@ VAR "z")) = 
+   LAM z (VAR "x" @@ VAR z @@ (VAR "y" @@ VAR z))`
+     by SRW_TAC [][LAM_eq_thm] THEN 
+  POP_ASSUM SUBST1_TAC THEN 
+  Q_TAC (NEW_TAC "y") `{"x"; "y"; z} ∪ FV M ∪ FV N` THEN 
+  `LAM "y" (LAM z (VAR "x" @@ VAR z @@ (VAR "y" @@ VAR z))) =
+   LAM y (LAM z (VAR "x" @@ VAR z @@ (VAR y @@ VAR z)))`
+     by SRW_TAC [][LAM_eq_thm] THEN 
+  POP_ASSUM SUBST1_TAC THEN 
+  ASM_SIMP_TAC (bsrw_ss()) [NOT_IN_SUB] THEN 
+  `∀x y. (x = y) ⇒ (x == y)` by SRW_TAC [][] THEN POP_ASSUM MATCH_MP_TAC THEN 
+  SRW_TAC [boolSimps.CONJ_ss][LAM_eq_thm, tpm_fresh, NOT_IN_SUB] THEN 
+  SRW_TAC [][GSYM fresh_tpm_subst, tpm_flip_args]);
+
+val I_I = store_thm(
+  "I_I",
+  ``LAM x (VAR x) = I``,
+  SIMP_TAC (srw_ss()) [LAM_eq_thm, chap2Theory.I_def]);
+
+val K_I = store_thm(
+  "K_I", 
+  ``v ∉ FV M ⇒ (LAM v M == K @@ M)``,
+  STRIP_TAC THEN REWRITE_TAC [chap2Theory.K_def] THEN 
+  Q_TAC (NEW_TAC "y") `{"x"; "y"} ∪ FV M` THEN 
+  `LAM "y" (VAR "x") = LAM y (VAR "x")` by SRW_TAC [][LAM_eq_thm] THEN 
+  POP_ASSUM SUBST1_TAC THEN 
+  ASM_SIMP_TAC (bsrw_ss()) [] THEN 
+  `∀x y. (x = y) ⇒ (x == y)` by SRW_TAC [][] THEN POP_ASSUM MATCH_MP_TAC THEN 
+  SRW_TAC [boolSimps.CONJ_ss][LAM_eq_thm, tpm_fresh, NOT_IN_SUB]);
+
+val S_I = store_thm(
+  "S_I",
+  ``v ∈ FV M ∧ v ∈ FV N ∧ N ≠ VAR v ⇒ 
+    LAM v (M @@ N) == S @@ (LAM v M) @@ (LAM v N)``,
+  STRIP_TAC THEN REWRITE_TAC [chap2Theory.S_def] THEN 
+  Q_TAC (NEW_TAC "z") `{"x"; "y"; "z"} ∪ FV M ∪ FV N` THEN 
+  `LAM "z" (VAR "x" @@ VAR "z" @@ (VAR "y" @@ VAR "z")) = 
+   LAM z (VAR "x" @@ VAR z @@ (VAR "y" @@ VAR z))`
+     by SRW_TAC [][LAM_eq_thm] THEN 
+  POP_ASSUM SUBST1_TAC THEN 
+  Q_TAC (NEW_TAC "y") `{"x"; "y"; z} ∪ FV M ∪ FV N` THEN 
+  `LAM "y" (LAM z (VAR "x" @@ VAR z @@ (VAR "y" @@ VAR z))) =
+   LAM y (LAM z (VAR "x" @@ VAR z @@ (VAR y @@ VAR z)))`
+     by SRW_TAC [][LAM_eq_thm] THEN 
+  POP_ASSUM SUBST1_TAC THEN 
+  ASM_SIMP_TAC (bsrw_ss()) [NOT_IN_SUB] THEN 
+  `LAM v (M @@ N) = LAM z ([VAR z/v] (M @@ N))`
+     by SRW_TAC [][SIMPLE_ALPHA] THEN 
+  SRW_TAC [][]);
+
+val fake_eta = store_thm(
+  "fake_eta",
+  ``v ∉ FV M ∧ is_abs M ⇒ (LAM v (M @@ VAR v) == M)``,
+  STRIP_TAC THEN 
+  `∃u M0. M = LAM u M0`
+     by (Q.SPEC_THEN `M` FULL_STRUCT_CASES_TAC term_CASES THEN 
+         FULL_SIMP_TAC (srw_ss()) [] THEN METIS_TAC []) THEN 
+  ASM_SIMP_TAC (bsrw_ss()) [] THEN 
+  FULL_SIMP_TAC (srw_ss()) [] THEN 
+  Cases_on `v = u` THEN SRW_TAC [][] THEN RES_TAC THEN 
+  `LAM u M0 = LAM v ([VAR v/u] M0)` by SRW_TAC [][SIMPLE_ALPHA] THEN 
+  SRW_TAC [][]);
+
+val is_abs_cfstsnd = Store_thm(
+  "is_abs_cfstsnd",
+  ``is_abs csnd ∧ is_abs cfst``,
+  SRW_TAC [][churchpairTheory.cfst_def, churchpairTheory.csnd_def]);
+
+val B_eta = store_thm(
+  "B_eta",
+  ``LAM v (B @@ VAR v) == B``,
+  SIMP_TAC (bsrw_ss()) [chap2Theory.B_def] THEN 
+  `S @@ (K @@ S) @@ K =
+   LAM "x" (LAM "y" (LAM "z" (VAR "x" @@ VAR "z" @@ (VAR "y" @@ VAR "z")))) @@ 
+       (K @@ S) @@ K`
+     by SRW_TAC [][chap2Theory.S_def] THEN 
+  ASM_SIMP_TAC (bsrw_ss()) [] THEN 
+  `∀x y. (x = y) ⇒ x == y` by SRW_TAC [][] THEN 
+  POP_ASSUM MATCH_MP_TAC THEN 
+  SRW_TAC [][LAM_eq_thm, tpm_fresh]);
+
+val eqn_elim = prove(
+  ``(∀Y. X:term == Y ⇔ Z == Y) ⇒ X == Z``,
+  METIS_TAC [chap2Theory.lam_eq_rules]);
+fun brackabs_equiv ths def = let 
+  val (l,r) = dest_eq (concl def)
+  val gv = genvar ``:term``
+  val t = ``^l == ^gv``
+  val th = SIMP_CONV (bsrw_ss()) 
+                     ([S_I, K_I, B_I, C_I, fake_eta, B_eta, I_I, def] @ ths)
+                     t
+in
+  MATCH_MP eqn_elim (GEN gv th) 
+end
+  
+val is_abs_cdV = Store_thm(
+  "is_abs_cdV",
+  ``is_abs cdV``,
+  SRW_TAC [][cdV_def]);
+val is_abs_cdAPP = Store_thm(
+  "is_abs_cdAPP",
+  ``is_abs cdAPP``,
+  SRW_TAC [][cdAPP_def]);
+
+val termrec_var_def = Define`
+  termrec_var = B @@ (S @@ (B @@ cpair @@ cdV)) @@ I
+`;
+val termrec_var_eta = store_thm(
+  "termrec_var_eta",
+  ``LAM x (termrec_var @@ VAR x) == termrec_var``,
+  SIMP_TAC (bsrw_ss()) [termrec_var_def] THEN 
+  CONV_TAC (RAND_CONV (SIMP_CONV bool_ss [Once chap2Theory.B_def])) THEN 
+  SIMP_TAC (bsrw_ss()) [] THEN 
+  CONV_TAC (RAND_CONV (SIMP_CONV bool_ss [Once chap2Theory.S_def])) THEN 
+  SIMP_TAC (bsrw_ss()) [] THEN 
+  `∀x y. (x = y) ⇒ x == y` by SRW_TAC [][] THEN 
+  POP_ASSUM MATCH_MP_TAC THEN 
+  SRW_TAC [][LAM_eq_thm, tpm_fresh]);  
+  
+
+val termrec_comb_def = Define`
+  termrec_comb = 
+  LAM "c" (LAM "r1" (LAM "r2" 
+    (cpair @@ (cdAPP @@ (cfst @@ VAR "r1") @@ (cfst @@ VAR "r2"))
+           @@ (VAR "c" 
+                   @@ (cfst @@ VAR "r1") @@ (cfst @@ VAR "r2")
+                   @@ (csnd @@ VAR "r1") @@ (csnd @@ VAR "r2")))))
+`;
+val termrec_comb_eqn = brackabs_equiv [] termrec_comb_def
+
+
+val termrec_abs_def = Define`
+  termrec_abs = 
+  LAM "a" (LAM "r" 
+    (cpair @@ (cdABS @@ (cfst @@ VAR "r"))
+           @@ (VAR "a" @@ (cfst @@ VAR "r") @@ (csnd @@ VAR "r"))))
+`;
+val termrec_abs_eqn = brackabs_equiv [] termrec_abs_def
+
+val FV_termrec_subs = Store_thm(
+  "FV_termrec_subs",
+  ``(FV termrec_var = {}) ∧ (FV termrec_comb = {}) ∧ (FV termrec_abs = {})``,
+  SRW_TAC [][termrec_var_def, termrec_comb_def, termrec_abs_def, EXTENSION]);
+
+val is_abs_termrecsubs = Store_thm(
+  "is_abs_termrecsubs",
+  ``is_abs termrec_comb ∧ is_abs termrec_abs``,
+  SRW_TAC [][termrec_var_def, termrec_comb_def, termrec_abs_def]);
+
+val fst_termrec_subs = store_thm(
+  "fst_termrec_subs",
+  ``∀t. cfst @@ (cDB t 
+                     @@ (termrec_var @@ v) 
+                     @@ (termrec_comb @@ c)
+                     @@ (termrec_abs @@ a)) == 
+        cDB t``,
+  SIMP_TAC (bsrw_ss()) [termrec_var_def, termrec_comb_eqn, termrec_abs_eqn] THEN
+  Induct THEN ASM_SIMP_TAC (bsrw_ss()) [cDB_thm, 
+                                        churchpairTheory.cfst_pair, 
+                                        cdV_behaviour, cdAPP_behaviour, 
+                                        cdABS_behaviour]);
+
+val termrec_def = Define`
+  termrec = 
+  LAM "v" (LAM "c" (LAM "a" (LAM "t"
+    (csnd @@ (VAR "t" 
+                  @@ (termrec_var @@ VAR "v")
+                  @@ (termrec_comb @@ VAR "c")
+                  @@ (termrec_abs @@ VAR "a"))))))
+`;
+
+val termrec_eqn = brackabs_equiv [termrec_var_eta] termrec_def
+
+val FV_termrec = Store_thm(
+  "FV_termrec",
+  ``FV termrec = {}``,
+  SRW_TAC [][termrec_def, EXTENSION]);
+
+infix |> fun x |> f = f x
+
+val termrec_behaviour = store_thm(
+  "termrec_behaviour",
+  ``termrec @@ v @@ c @@ a @@ cDB (dV i) == v @@ church i ∧
+    termrec @@ v @@ c @@ a @@ cDB (dAPP t u) ==
+      c @@ cDB t @@ cDB u 
+        @@ (termrec @@ v @@ c @@ a @@ cDB t)
+        @@ (termrec @@ v @@ c @@ a @@ cDB u) ∧
+    termrec @@ v @@ c @@ a @@ cDB (dABS t) ==
+      a @@ cDB t @@ (termrec @@ v @@ c @@ a @@ cDB t)``,
+  REPEAT CONJ_TAC THENL [
+    SIMP_TAC (bsrw_ss()) [termrec_eqn, cDB_thm, termrec_var_def, 
+                          churchpairTheory.csnd_pair],
+
+    SIMP_TAC (bsrw_ss()) [termrec_eqn, cDB_thm] THEN 
+    ASSUME_TAC (``termrec_comb @@ c @@ x @@ y == X`` 
+                  |> SIMP_CONV (bsrw_ss()) [termrec_comb_eqn]
+                  |> Q.GEN `X`
+                  |> MATCH_MP eqn_elim 
+                  |> Q.GEN `y` |> Q.GEN `x`) THEN 
+    ASM_SIMP_TAC (bsrw_ss()) [churchpairTheory.csnd_pair, fst_termrec_subs],
+    
+    SIMP_TAC (bsrw_ss()) [termrec_eqn, cDB_thm] THEN 
+    ASSUME_TAC (``termrec_abs @@ a @@ x == X`` 
+                  |> SIMP_CONV (bsrw_ss()) [termrec_abs_eqn]
+                  |> Q.GEN `X`
+                  |> MATCH_MP eqn_elim 
+                  |> Q.GEN `x`) THEN 
+    ASM_SIMP_TAC (bsrw_ss()) [churchpairTheory.csnd_pair, fst_termrec_subs]
+  ]);
   
 (* ---------------------------------------------------------------------- 
     cichurch 
@@ -423,96 +665,161 @@ val ccDB_behaviour = store_thm(
   Q.SPEC_THEN `dbt` ASSUME_TAC cDB_def THEN 
   SRW_TAC [][]);
 
-open normal_orderTheory
-
 (* ---------------------------------------------------------------------- 
-    Halting Problems.
-
-    HP_selfapp is where a diagonalisation is done.  This is usually
-    done by saying something like there is no computable function for
-    determining if φ_n(n) terminates.  One reads this with "n" as the
-    starting point, and this then leading to the use of φ_n to apply
-    to it.
-  
-    But equally, we know that every f has an index, and this says that
-    if you apply an f to its index, then the thing is undecidable.  In
-    the λ-calculus setting, the cDB function is the function that
-    takes a term to its "index", where here, the "index" is the data
-    encoding the function.
-
-    So, this proof is easiest to read as saying, given a term f, it's
-    impossible to determine if it applied to its index halts.
-  
-    Will perhaps add a more traditional looking version with natural
-    numbers too.
+    enumerations are computable 
    ---------------------------------------------------------------------- *)
 
-val HP_selfapp = store_thm(
-  "HP_selfapp",
-  ``¬∃M. 
-         ∀t. M @@ cDB (fromTerm t) -n->* 
-             cB (has_bnf (t @@ cDB (fromTerm t)))``,
-  STRIP_TAC THEN 
-  FULL_SIMP_TAC (srw_ss()) [] THEN 
-  Q_TAC (NEW_TAC "z") `FV M` THEN 
-  Q.ABBREV_TAC `G = LAM z (M @@ VAR z @@ Ω @@ cB T)` THEN 
-  `G @@ cDB (fromTerm G) -β-> M @@ cDB (fromTerm G) @@ Ω @@ cB T`
-      by SRW_TAC [][chap3Theory.ccbeta_rwt, lemma14b, Abbr`G`] THEN 
-  `M @@ cDB (fromTerm G) @@ Ω @@ cB T 
-      -β->* 
-   cB (has_bnf (G @@ cDB (fromTerm G))) @@ Ω @@ cB T`
-      by SRW_TAC [][chap3Theory.betastar_APPl, nstar_betastar] THEN 
-  Cases_on `has_bnf (G @@ cDB (fromTerm G))` THEN 
-  FULL_SIMP_TAC (srw_ss()) [] THENL [
-    `cB T @@ Ω @@ cB T -β->* Ω`
-       by SRW_TAC [][nstar_betastar, cB_behaviour] THEN 
-    `G @@ cDB (fromTerm G) -β->* Ω`
-       by METIS_TAC [relationTheory.RTC_RULES, 
-                     relationTheory.RTC_CASES_RTC_TWICE] THEN 
-    METIS_TAC [Omega_reachable_no_bnf],
+open enumerationsTheory
 
-    `cB F @@ Ω @@ cB T -β->* cB T`
-       by SRW_TAC [][nstar_betastar, cB_behaviour] THEN 
-    `G @@ cDB (fromTerm G) -β->* cB T`
-       by METIS_TAC [relationTheory.RTC_CASES_RTC_TWICE, 
-                     relationTheory.RTC_RULES] THEN 
-    `has_bnf (G @@ cDB (fromTerm G))`
-       by METIS_TAC [chap3Theory.has_bnf_thm, bnf_cB]
+
+
+
+val cdBnum_def = Define`
+  cdBnum = 
+  LAM "t" 
+    (VAR "t" 
+         @@ (cmult @@ church 3)
+         @@ (LAM "r1" 
+               (B @@ csuc 
+                  @@ (B @@ (cmult @@ church 3) 
+                        @@ (cnpair @@ VAR "r1"))))
+         @@ (B @@ (cplus @@ church 2) @@ (cmult @@ church 3)))
+`;
+
+val FV_cdBnum = Store_thm(
+  "FV_cdBnum",
+  ``FV cdBnum = {}``,
+  SRW_TAC [][cdBnum_def]);
+
+val cdBnum_behaviour = store_thm(
+  "cdBnum_behaviour",
+  ``cdBnum @@ cDB t -n->* church (dBnum t)``,
+  SIMP_TAC (bsrw_ss()) [cdBnum_def] THEN Induct_on `t` THEN 
+  ASM_SIMP_TAC (bsrw_ss() ++ ARITH_ss) 
+               [cDB_thm, dBnum_def, cmult_behaviour, 
+                cnpair_behaviour, csuc_behaviour, 
+                arithmeticTheory.ADD1, cplus_behaviour]);
+
+val cndbsuc_def = Define`
+  cndbsuc = 
+  LAM "r" (LAM "n" (LAM "m3" (LAM "d3"
+             (cis_zero @@ VAR "m3"
+              @@ (cdV @@ VAR "d3")
+              @@ (ceqnat @@ VAR "m3" @@ (church 1)
+                         @@ (cdAPP @@ (VAR "r" @@ (cnfst @@ VAR "d3"))
+                                   @@ (VAR "r" @@ (cnsnd @@ VAR "d3")))
+                         @@ (cdABS @@ (VAR "r" @@ VAR "d3")))))
+            @@ (cmod @@ VAR "n" @@ church 3)
+            @@ (cdiv @@ VAR "n" @@ church 3)))
+`;
+val FV_cndbsuc = Store_thm(
+  "FV_cndbsuc",
+  ``FV cndbsuc = {}``,
+  SRW_TAC [][cndbsuc_def, EXTENSION]);
+
+val cndbsuc_dV_behaviour = store_thm(
+  "cndbsuc_dV_behaviour",
+  ``(n MOD 3 = 0) ⇒ 
+    cndbsuc @@ r @@ church n -n->* cDB (dV (n DIV 3))``,
+  SIMP_TAC (bsrw_ss()) [cndbsuc_def] THEN FRESH_TAC THEN 
+  ASM_SIMP_TAC (bsrw_ss()) [tpm_fresh, cmod_behaviour, cis_zero_behaviour, 
+                            cB_behaviour, cdiv_behaviour, cdV_behaviour]);
+
+
+val is_abs_cmoddiv = Store_thm(
+  "is_abs_cmoddiv",
+  ``is_abs cmod ∧ is_abs cdiv``,
+  SRW_TAC [][cmod_def, cdiv_def]);
+
+val cndbsuc_eqn = brackabs_equiv [] cndbsuc_def
+
+val cndbsuc_dAPP_behaviour = store_thm(
+  "cndbsuc_dAPP_behaviour",
+  ``(n MOD 3 ≠ 0) ∧ (n MOD 3 = 1) ⇒ 
+    cndbsuc @@ r @@ church n == 
+    cdAPP @@ (r @@ (cnfst @@ church (n DIV 3))) 
+          @@ (r @@ (cnsnd @@ church (n DIV 3)))``,
+  STRIP_TAC THEN 
+  ASM_SIMP_TAC (bsrw_ss()) [cndbsuc_eqn, cmod_behaviour, cis_zero_behaviour, 
+                            ceqnat_behaviour, cB_behaviour, cdiv_behaviour]);
+
+val cndbsuc_dABS_behaviour = store_thm(
+  "cndbsuc_dABS_behaviour",
+  ``(n MOD 3 ≠ 0) ∧ (n MOD 3 ≠ 1) ⇒
+    cndbsuc @@ r @@ church n == cdABS @@ (r @@ church (n DIV 3))``,
+  STRIP_TAC THEN 
+  ASM_SIMP_TAC (bsrw_ss()) [cndbsuc_eqn, cmod_behaviour, cis_zero_behaviour, 
+                            ceqnat_behaviour, cB_behaviour, cdiv_behaviour]);
+ 
+val cnumdB0_def = Define`
+  cnumdB0 = 
+  natrec 
+   @@ (LAM "n" (cDB (dV 0)))
+   @@ (LAM "c0" (LAM "r" (LAM "n"
+       (ceqnat @@ (csuc @@ VAR "c0") @@ (VAR "n")
+        @@ (cndbsuc @@ VAR "r" @@ VAR "n")
+        @@ (VAR "r" @@ VAR "n")))))
+`;
+        
+val FV_cnumdB0 = Store_thm(
+  "FV_cnumdB0",
+  ``FV cnumdB0 = {}``,
+  SRW_TAC [][cnumdB0_def, EXTENSION])
+
+val cnumdB0_behaviour = store_thm(
+  "cnumdB0_behaviour",
+  ``n ≤ c ⇒ cnumdB0 @@ church c @@ church n -n->* cDB (numdB n)``,
+  Q.ID_SPEC_TAC `n` THEN SIMP_TAC (bsrw_ss()) [cnumdB0_def] THEN 
+  Induct_on `c` THEN
+  SIMP_TAC (bsrw_ss()) [natrec_behaviour, cdV_behaviour, 
+                        csuc_behaviour, cmod_behaviour, cdiv_behaviour, 
+                        ceqnat_behaviour] 
+  THEN1 SRW_TAC [][Once numdB_def] THEN 
+  REPEAT STRIP_TAC THEN Q.ABBREV_TAC `N = SUC c` THEN 
+  Cases_on `n = N` THENL [
+    SRW_TAC [][] THEN 
+    ASM_SIMP_TAC (bsrw_ss()) [cB_behaviour] THEN 
+    Cases_on `N MOD 3 = 0` THENL [
+      ASM_SIMP_TAC (bsrw_ss()) [cndbsuc_dV_behaviour] THEN 
+      ASM_SIMP_TAC (srw_ss()) [Once numdB_def],
+
+      `0 < N` by SRW_TAC [][Abbr`N`] THEN 
+      `N DIV 3 < N` 
+        by SRW_TAC [ARITH_ss][arithmeticTheory.DIV_LESS] THEN 
+      `N DIV 3 ≤ c` by SRW_TAC [ARITH_ss][Abbr`N`] THEN 
+      Cases_on `N MOD 3 = 1` THENL [
+        ASM_SIMP_TAC (bsrw_ss()) [cndbsuc_dAPP_behaviour, Once numdB_def] THEN 
+        `nsnd (N DIV 3) ≤ c ∧ nfst (N DIV 3) ≤ c`
+           by (ASSUME_TAC (Q.INST [`n` |-> `N DIV 3`] 
+                                  numpairTheory.nsnd_le) THEN
+               ASSUME_TAC (Q.INST [`n` |-> `N DIV 3`] 
+                                  numpairTheory.nfst_le) THEN
+               DECIDE_TAC) THEN 
+        ASM_SIMP_TAC (bsrw_ss()) [cnfst_behaviour, cnsnd_behaviour, 
+                                  cdAPP_behaviour],
+
+        ASM_SIMP_TAC (bsrw_ss()) [cndbsuc_dABS_behaviour, Once numdB_def, 
+                                  cdABS_behaviour]
+      ]
+    ],
+
+    ASM_SIMP_TAC (bsrw_ss()) [cB_behaviour] THEN 
+    `n ≤ c` by SRW_TAC [ARITH_ss][Abbr`N`] THEN 
+    ASM_SIMP_TAC (bsrw_ss()) []
   ]);
 
-(* Impossibility of determining whether or not arbitrary function applied
-   to arbitrary argument will terminate. *)    
-val HP_fx = store_thm(
-  "HP_fx",
-  ``¬∃M. ∀f x. M @@ cDB (fromTerm f) @@ x -n->* cB (has_bnf (f @@ x))``,
-  STRIP_TAC THEN Q_TAC (NEW_TAC "z") `FV M` THEN 
-  Q.ABBREV_TAC `G = LAM z (M @@ VAR z @@ VAR z)` THEN 
-  `∀t. G @@ cDB (fromTerm t) -n-> M @@ cDB (fromTerm t) @@ cDB (fromTerm t)`
-      by SRW_TAC [][noreduct_characterisation, noreduct_thm, Abbr`G`, 
-                    lemma14b] THEN 
-  `∀t. M @@ cDB (fromTerm t) @@ cDB (fromTerm t) -n->* 
-       cB (has_bnf (t @@ cDB (fromTerm t)))` 
-      by SRW_TAC [][] THEN 
-  `∀t. G @@ cDB (fromTerm t) -n->* cB (has_bnf (t @@ cDB (fromTerm t)))`
-     by METIS_TAC [relationTheory.RTC_RULES] THEN 
-  METIS_TAC [HP_selfapp]);
+val cnumdB_def = Define`
+  cnumdB = LAM "n" (cnumdB0 @@ VAR "n" @@ VAR "n")
+`; 
 
-(* Impossibility of deciding whether or not an arbitrary term has a β-nf.
-   Needs the computability of the encoding function cDB. *)
-val HP_bnf = store_thm(
-  "HP_bnf",
-   ``¬∃M. ∀t. M @@ cDB (fromTerm t) -n->* cB (has_bnf t)``,
-  STRIP_TAC THEN Q_TAC (NEW_TAC "z") `FV M` THEN 
-  Q.ABBREV_TAC `G = LAM z (M @@ (cdAPP @@ VAR z @@ (ccDB @@ VAR z)))` THEN 
-  `∀t. G @@ cDB (fromTerm t) -n->* cB (has_bnf (t @@ cDB (fromTerm t)))`
-    by (ASM_SIMP_TAC (bsrw_ss()) [Abbr`G`, cdAPP_behaviour, 
-                                  ccDB_behaviour] THEN 
-        REPEAT GEN_TAC THEN 
-        `∀f x. dAPP (fromTerm f) (fromTerm x) = fromTerm (f @@ x)`
-           by SRW_TAC [][] THEN 
-        ASM_SIMP_TAC (betafy bool_ss) [] THEN 
-        MATCH_MP_TAC nstar_betastar THEN ASM_SIMP_TAC (srw_ss()) []) THEN 
-  METIS_TAC [HP_selfapp]);
+val FV_cnumdB = Store_thm(
+  "FV_cnumdB",
+  ``FV cnumdB = {}``,
+  SRW_TAC [][cnumdB_def]);
+
+val cnumdB_behaviour = store_thm(
+  "cnumdB_behaviour",
+  ``cnumdB @@ church n -n->* cDB (numdB n)``,
+  SIMP_TAC (bsrw_ss()) [cnumdB_def, cnumdB0_behaviour]);
   
-
 val _ = export_theory()
